interpreter.v
@@ -27,12 +27,12 @@ Context (e : state Ti → list E).
 Let interpreter_env := (natural_env ptr_size align_base).
 Existing Instance interpreter_env.
 
-Definition cstep_exec' (Γ : env Ti) (δ : funenv Ti)
+Definition cexec' (Γ : env Ti) (δ : funenv Ti)
     (iS : istate Ti E) : listset (istate Ti E) :=
   let (_,εs,S) := iS in
   (λ S_new,
     let εs_new := e S_new in IState εs_new (εs ++ εs_new) S_new
-  ) <$> cstep_exec Γ δ S.
+  ) <$> cexec Γ δ S.
 Definition interpreter_initial
     (Θ : list (N * decl Ti)) (f : funname) (ces : list (cexpr Ti)) :
     string + (env Ti * funenv Ti * istate Ti E) :=
@@ -49,15 +49,15 @@ Definition interpreter_initial
   inr (Γ, δ, IState [] [] (initial_state m f vs)).
 
 Context (hash : istate Ti E → Z).
-Definition cstep_exec_all (Γ : env Ti) (δ : funenv Ti) (iS : istate Ti E) :
+Definition cexec_all (Γ : env Ti) (δ : funenv Ti) (iS : istate Ti E) :
     listset (istate Ti E) * listset (istate Ti E) :=
-  let nexts := cstep_exec' Γ δ iS in
+  let nexts := cexec' Γ δ iS in
   if decide (nexts ≡ ∅) then (∅, {[ iS ]}) else (nexts, ∅).
 Definition csteps_exec_all (Γ : env Ti) (δ : funenv Ti) :
     listset (istate Ti E) →
     stream (listset (istate Ti E) * listset (istate Ti E)) :=
   cofix go iSs :=
-  let nexts := cstep_exec_all Γ δ <$> iSs in
+  let nexts := cexec_all Γ δ <$> iSs in
   let reds := listset_normalize hash (nexts ≫= fst) in
   let nfs := listset_normalize hash (nexts ≫= snd) in
   (reds,nfs) :.: go reds.
@@ -73,7 +73,7 @@ Context (rand : nat → nat).
 Definition csteps_exec_rand (Γ : env Ti) (δ : funenv Ti) :
     istate Ti E → stream (istate Ti E + istate Ti E) :=
   cofix go iS :=
-  match listset_car (cstep_exec' Γ δ iS) with
+  match listset_car (cexec' Γ δ iS) with
   | [] => srepeat (inr iS)
   | (iS' :: _) as iSs =>
      let next := from_option iS' (iSs !! rand (length iSs)) in
